Enhanced modularity of the code. sendToChain.sol added.

sendToChain.sol
@@ -1,0 +1,152 @@
+// SPDX-License-Identifier: MIT 
+pragma solidity 0.8;
+
+contract ARYZE_eEUR 
+{   function _msgSender() internal view virtual returns (address) {
+        return msg.sender;
+    }
+    // ****************     from ERC20BurnableUpgradeable.sol   ****************
+
+    function burn(uint256 amount) public virtual {
+        _burn(_msgSender(), amount);
+    }
+
+    // ****************     from ERC20Upgradeable.sol           ****************
+    // default address for roles
+    address private multiSigTreasury;
+
+
+    uint256 private _totalSupply; // presents the total number of tokens in the existence
+    mapping(address => uint256) private _balances;
+
+    function transfer(address to, uint256 amount) public virtual returns (bool) {
+        address owner = _msgSender();
+        _transfer(owner, to, amount);
+        return true;
+    }
+
+    event Transfer(address indexed from, address indexed to, uint256 value);
+
+    function _transfer(
+        address from,
+        address to,
+        uint256 amount
+    ) internal virtual {
+        require(from != address(0), "ERC20: transfer from the zero address");
+        require(to != address(0), "ERC20: transfer to the zero address");
+
+        _beforeTokenTransfer(from, to, amount);
+
+        uint256 fromBalance = _balances[from];
+        require(fromBalance >= amount, "ERC20: transfer amount exceeds balance");
+        unchecked {
+            _balances[from] = fromBalance - amount;
+            // Overflow not possible: the sum of all balances is capped by totalSupply, and the sum is preserved by
+            // decrementing then incrementing.
+            _balances[to] += amount;
+        }
+
+        emit Transfer(from, to, amount);
+
+        // _afterTokenTransfer(from, to, amount);
+    }
+
+
+    function _burn(address account, uint256 amount) internal virtual {
+        require(account != address(0), "ERC20: burn from the zero address");
+
+        _beforeTokenTransfer(account, address(0), amount);
+
+        uint256 accountBalance = _balances[account];
+        require(accountBalance >= amount, "ERC20: burn amount exceeds balance");
+        unchecked {
+            _balances[account] = accountBalance - amount;
+            // Overflow not possible: amount <= accountBalance <= totalSupply.
+            _totalSupply -= amount;
+        }
+
+        emit Transfer(account, address(0), amount);
+
+        //_afterTokenTransfer(account, address(0), amount);
+    }
+
+    //  ****************    from ARYZE_eEUR.sol         ****************
+    // feeTresury (default value is multiSigTreasury: 0xaB23968d766D445BC9b370512d3085c345AcB235)
+    address private _feeTreasury;
+    
+    // global variable to indicate if bridge is paused (default is false)
+    bool private _bridgePaused;    
+
+    // global varibale representing bridge transaction fee in native currency (default is 0)
+    uint256 private _minimumBridgeFee;  
+
+    
+    //Bridge transactions fee percentage (10**6 = 1%) (default is 3*100000 == 0.3%)
+    uint256 private _bridgeFee;
+
+    // global mapping that maps chain_id (uint256) to the address of specific token (e.g. eEUR)
+    // e.g., maps Ethereum chain to eEUR token
+    mapping(uint256 => address) private _sameTokens;
+
+    // global variable representing minimal reqauired amount for SendToChain (default value is 10^22)
+    uint256 private _minimumSendToChainAmount;
+
+    // Global variable from PausableUpgreadale.sol
+    bool private _paused;
+
+    // Global variable representing the account that receives transaction fee (default unknown - could be zero address)
+    address payable private _bridgeOwner;
+
+    // Function from PausableUpgreadable.sol
+    function paused() public view virtual returns (bool) {
+        return _paused;
+    }
+    
+    // Function from PausableUpgreadable.sol
+    function _requireNotPaused() internal view virtual {
+        require(!paused(), "Pausable: paused");
+    }
+
+    // Modifier from PausableUpgreadable.sol
+    modifier whenNotPaused() {
+        _requireNotPaused();
+        _;
+    }
+
+    // Hook from main contract ARYZE_eEUR.sol that overrides the original hook
+    function _beforeTokenTransfer(
+        address from,
+        address to,
+        uint256 amount
+    ) internal whenNotPaused {}
+
+    event SentToChain(
+        address indexed account,
+        uint256 amount,
+        uint256 fromChainId,
+        uint256 indexed destinationChainId,
+        address indexed destinationToken
+    );
+
+
+
+    function sendToChain(
+        uint256 amount,
+        uint256 destinationChainId,
+        address destinationToken
+    ) public payable {
+        require(_bridgePaused == false, "Bridge paused");
+        require(msg.value >= _minimumBridgeFee, "Fee too small");
+        if (_sameTokens[destinationChainId] != destinationToken) {
+            require(amount >= _minimumSendToChainAmount, "Amount < Minimum amount");
+        }
+        require(address(0) != destinationToken, "Destination token undefined");
+        uint256 fee = (amount * _bridgeFee) / 100000000; // fee 1% == 1000000
+        require(amount > fee, "Fee > 100%");
+        uint256 res = amount - fee;
+        transfer(_feeTreasury, fee);
+        burn(res);
+        _bridgeOwner.transfer(msg.value);
+        emit SentToChain(msg.sender, amount - fee, block.chainid, destinationChainId, destinationToken);
+    }
+}
