CommonFunctions.fst
@@ -1,0 +1,26 @@
+module CommonFunctions
+
+open Solidity
+open GlobalState
+
+(* function that checks if specific account has specific role assgined to them
+   from `eEUR_AccessControlUpgredeable.sol` *)
+let hasRole     (state: global_state)
+                (input_role: string_66)
+                (account: address)
+                : bool =
+     Solidity.get (Solidity.get state._roles input_role).members account  
+     // returns bool from mapping => `return _roles[role].members[account];`   
+
+(*  function returns current value of global variable `_paused`  *)
+let paused      (state: global_state)
+                : bool =
+                state._paused
+
+(*  check if addition of two uints results in overflow
+    e.g., in _mint => x = _totalSupply and y = amount
+ *)
+let overflow_check (x:uint) (y:uint) : option uint =
+    // checks if (uint_max - x) < y ==> overflow
+    if UInt256.lt (UInt256.sub Solidity.max_uint x) y then None 
+    else Some (UInt256.add x y) // overflow not possible!
