GlobalState.fst
@@ -1,0 +1,97 @@
+module GlobalState
+open Solidity
+open FStar.String
+
+(* 
+    New type string_66 that only allows strings with 66 characters
+    effectively simulating hexadecimal number of length 64 (+ '0x') == 256 bit number
+*)
+type string_66 = s:string {length s = 66}   // another way to represent 32byte values
+
+let default_string_66 : string_66 = 
+    let def_str = "0x0000000000000000000000000000000000000000000000000000000000000000" in
+    let _ = assume(String.length def_str = 66) in 
+    def_str
+// Add relevant event for reforge
+// event Reforged(address indexed account, uint256 amount, string indexed transaction);
+// event Transfer(address indexed from, address indexed to, uint256 value);
+type event = 
+    | Reforged : address -> uint -> string_66 -> event
+    | Transfer : address -> address -> uint -> event
+
+(*
+Add all possible roles (they have type string_66 since keccak256 returns hash - hex number of lenght 64)
+*)
+(*
+type role =  
+	| PAUSER_ROLE        : string_66 -> role
+	| MINTER_ROLE        : string_66 -> role
+	| UPGRADER_ROLE      : string_66 -> role
+	| BRIDGE_OWNER_ROLE  : string_66 -> role
+    | ADMIN_eEUR         : string_66 -> role
+*)
+type role = { 
+	_PAUSER_ROLE        : string_66;
+	_MINTER_ROLE        : string_66;
+	_UPGRADER_ROLE      : string_66; 
+	_BRIDGE_OWNER_ROLE  : string_66;
+    _ADMIN_eEUR         : string_66;
+}
+
+(*
+Struct from `eEUR_AccessControlUpgreadable.sol` that defines if specific address 
+has assigned specific role (`true`) 
+*)
+noeq type _RoleData = {
+    members     : address -> bool;
+    adminRole   : string_66
+}
+
+noeq type global_state = {
+    (* list of events *)
+    events_         : list event;
+
+    (* mapping transaction string (transaction hash) to bool
+       bool is by default set to `false` *)
+    _transactions   : string_66 -> bool;
+
+    (* type that contains all role hashes (keccak256 hashes) *)
+    roles           : role;
+
+    (* mapping role hashes (keccak256 hashes) into _RoleData struct *)
+    _roles          : string_66 -> _RoleData;  
+
+    (* uint that presents the total number of tokens in the existence
+       essentially it presents all tokens that were ever minted *)
+    _totalSupply    : uint;
+
+    (* mapping address to uint (representing the balance of tokens for specific account) *)
+    _balances       : address -> uint;
+
+    (* address that receives transaction fees in native currency *)
+    _bridgeOwner    : address;
+
+    (* boolean variable, indicates if contract is paused *)
+    _paused         : bool; 
+
+}
+
+let default_state : global_state = {
+    events_         = [];
+    _transactions   = ( fun x -> false );
+    roles           = {
+                        _PAUSER_ROLE        = default_string_66;
+                        _MINTER_ROLE        = default_string_66;
+                        _UPGRADER_ROLE      = default_string_66;
+                        _BRIDGE_OWNER_ROLE  = default_string_66;
+                        _ADMIN_eEUR         = default_string_66;
+    };
+    _roles          = ( fun role -> { 
+                                        members = ( fun addr -> false ); 
+                                        adminRole = default_string_66 
+                                    });    
+    _totalSupply    = Solidity.to_uint 0;
+    _balances       = ( fun x -> Solidity.to_uint 0   );
+    _bridgeOwner    = default_address;
+    _paused         = false;
+}
